Add test drive with basic Nat iota tests

Main.lean
@@ -356,38 +356,3 @@ unsafe def transCmd : Cmd := `[Cli|
 
 unsafe def main (args : List String) : IO UInt32 := do
   transCmd.validate args
-
-/- Theorems for patching iota reduction -/
-
-theorem nat_iota_zero {motive : Nat → Sort u} (zero : motive Nat.zero)
-  (succ : (n : Nat) → (ih : motive n) → motive (n.succ)) :
-  Nat.rec (motive := motive) zero succ 0 ≍ zero := by rfl
-
-theorem nat_iota_succ {motive : Nat → Sort u} (zero : motive Nat.zero)
-  (succ : (n : Nat) → (ih : motive n) → motive n.succ) (t : Nat) :
-  Nat.rec (motive := motive) zero succ t.succ ≍
-  succ t (Nat.rec (motive := motive) zero succ t) := by rfl
-
-/- Set up the information for using those iota reduction theorem -/
-
-def natIotaReductionData : IotaReductionData :=
-  (∅ : Std.HashMap Name Name)
-    |>.insert ``Nat.succ ``nat_iota_succ
-    |>.insert ``Nat.zero ``nat_iota_zero
-
-def iotaReduction : Std.HashMap Name IotaReductionData :=
-  (∅ : Std.HashMap Name IotaReductionData)
-  |>.insert ``Nat.rec natIotaReductionData
-
-/- Test patching iota reduction-/
-def motive := fun (_ : Nat) => Type
-def zero := Unit
-def succ (n : Nat) (_ : motive n) := Unit
-
-theorem test2 (f : Unit → False) (t : Nat.rec (motive := motive) zero succ 1) :
-  False := f t
-theorem test3 (f : Unit → False) (t : Nat.rec (motive := motive) zero succ 0) :
-  False := f t
-
-#patch_const test2 (iotaReduction := iotaReduction) -kLikeReduction -proofIrrelevance
-#patch_const test3 (iotaReduction := iotaReduction) -kLikeReduction -proofIrrelevance
