tests/NatIota.lean
@@ -1,0 +1,183 @@
+import Lean
+import Lean4Less.Commands
+import Lean4Less.Ext
+open Lean Lean4Less
+
+/- Theorems for patching iota reduction -/
+
+theorem nat_iota_zero {motive : Nat → Sort u} (zero : motive Nat.zero)
+  (succ : (n : Nat) → (ih : motive n) → motive (n.succ)) :
+  Nat.rec (motive := motive) zero succ 0 ≍ zero := by rfl
+
+theorem nat_iota_succ {motive : Nat → Sort u} (zero : motive Nat.zero)
+  (succ : (n : Nat) → (ih : motive n) → motive n.succ) (t : Nat) :
+  Nat.rec (motive := motive) zero succ t.succ ≍
+  succ t (Nat.rec (motive := motive) zero succ t) := by rfl
+
+/- Set up the information for using those iota reduction theorem -/
+
+def natIotaReductionData : IotaReductionData :=
+  (∅ : Std.HashMap Name Name)
+    |>.insert ``Nat.succ ``nat_iota_succ
+    |>.insert ``Nat.zero ``nat_iota_zero
+
+def iotaReduction : Std.HashMap Name IotaReductionData :=
+  (∅ : Std.HashMap Name IotaReductionData)
+  |>.insert ``Nat.rec natIotaReductionData
+
+/- Test patching iota reduction-/
+def motive := fun (_ : Nat) => Type
+def zero := Unit
+def succ (n : Nat) (_ : motive n) := Unit
+
+theorem test2 (f : Unit → False) (t : Nat.rec (motive := motive) zero succ 1) :
+  False := f t
+theorem test3 (f : Unit → False) (t : Nat.rec (motive := motive) zero succ 0) :
+  False := f t
+
+/--
+info: fun f t => f (L4L.castHEq (nat_iota_succ zero succ 0) t)
+-/
+#guard_msgs in
+#patch_const test2 (iotaReduction := iotaReduction) -kLikeReduction -proofIrrelevance
+
+/--
+info: fun f t => f (L4L.castHEq (nat_iota_zero zero succ) t)
+-/
+#guard_msgs in
+#patch_const test3 (iotaReduction := iotaReduction) -kLikeReduction -proofIrrelevance
+
+/--
+info: fun x x_1 x_2 =>
+  Nat.brecOn (motive := fun x => ∀ (x_3 : Nat), x ≤ x_3 → x = x_3 ∨ x < x_3) x
+    (fun x f x_3 x_4 =>
+      (match (motive :=
+          ∀ (x x_5 : Nat),
+            x ≤ x_5 →
+              ∀ (x_7 : Nat.below (motive := fun x => ∀ (x_7 : Nat), x ≤ x_7 → x = x_7 ∨ x < x_7) x), x = x_5 ∨ x < x_5)
+          x, x_3, x_4 with
+        | Nat.zero, Nat.zero, x => fun x => Or.inl rfl
+        | Nat.zero, n.succ, x => fun x => Or.inr (Nat.succ_le_succ (Nat.zero_le n))
+        | n.succ, Nat.zero, h => fun x => absurd h (Nat.not_succ_le_zero n)
+        | n.succ, m.succ, h => fun x =>
+          let this := Nat.le_of_succ_le_succ h;
+          match x.1 m this with
+          | Or.inl h => Or.inl (h ▸ rfl)
+          | Or.inr h =>
+            Or.inr
+              (L4L.castHEq
+                (L4L.appArgHEq' (fun n => n.le m.succ)
+                  (L4L.appArgHEq Nat.succ
+                    (L4L.appArgHEq Nat.succ
+                      (HEq.trans
+                        (L4L.appArgHEq' (fun f => f n)
+                          (L4L.appHEqABUV'
+                            (L4L.appArgHEq' (PProd ((fun x => Nat → Nat) 0))
+                              (nat_iota_zero PUnit fun n n_ih => (fun x => Nat → Nat) n ×' n_ih))
+                            (fun a a_1 a_2 =>
+                              L4L.HEqRefl
+                                ((fun β a => (fun x => Nat → Nat) 0) (Nat.below (motive := fun x => Nat → Nat) 0) a))
+                            (L4L.appArgHEq' ((fun α β a => a.1) ((fun x => Nat → Nat) 0))
+                              (nat_iota_zero PUnit fun n n_ih => (fun x => Nat → Nat) n ×' n_ih))
+                            (nat_iota_zero
+                              ⟨(fun x f x_5 =>
+                                    (match (motive :=
+                                        Nat → (x : Nat) → Nat.below (motive := fun x => Nat → Nat) x → Nat) x_5, x with
+                                      | a, Nat.zero => fun x => a
+                                      | a, b.succ => fun x => (x.1 a).succ)
+                                      f)
+                                  Nat.zero PUnit.unit,
+                                PUnit.unit⟩
+                              fun n n_ih =>
+                              ⟨(fun x f x_5 =>
+                                    (match (motive :=
+                                        Nat → (x : Nat) → Nat.below (motive := fun x => Nat → Nat) x → Nat) x_5, x with
+                                      | a, Nat.zero => fun x => a
+                                      | a, b.succ => fun x => (x.1 a).succ)
+                                      f)
+                                  n.succ n_ih,
+                                n_ih⟩)))
+                        (nat_iota_zero ((fun a x => a) n) fun n_1 n_ih =>
+                          (fun n_2 => (fun a b x => (x.1 a).succ) n n_2) n_1)))))
+                (Nat.succ_le_succ
+                  (L4L.castHEq
+                    (L4L.appArgHEq' (fun n => n.le m)
+                      (HEq.trans
+                        (L4L.appArgHEq Nat.succ
+                          (HEq.trans
+                            (nat_iota_zero ((fun a x => a) n) fun n_1 n_ih =>
+                              (fun n_2 => (fun a b x => (x.1 a).succ) n n_2) n_1)
+                            (L4L.appArgHEq' (fun f => f n)
+                              (HEq.symm
+                                (L4L.appHEqABUV'
+                                  (L4L.appArgHEq' (PProd ((fun x => Nat → Nat) 0))
+                                    (nat_iota_zero PUnit fun n n_ih => (fun x => Nat → Nat) n ×' n_ih))
+                                  (fun a a_1 a_2 =>
+                                    L4L.HEqRefl
+                                      ((fun β a => (fun x => Nat → Nat) 0) (Nat.below (motive := fun x => Nat → Nat) 0)
+                                        a))
+                                  (L4L.appArgHEq' ((fun α β a => a.1) ((fun x => Nat → Nat) 0))
+                                    (nat_iota_zero PUnit fun n n_ih => (fun x => Nat → Nat) n ×' n_ih))
+                                  (nat_iota_zero
+                                    ⟨(fun x f x_5 =>
+                                          (match (motive :=
+                                              Nat → (x : Nat) → Nat.below (motive := fun x => Nat → Nat) x → Nat) x_5,
+                                              x with
+                                            | a, Nat.zero => fun x => a
+                                            | a, b.succ => fun x => (x.1 a).succ)
+                                            f)
+                                        Nat.zero PUnit.unit,
+                                      PUnit.unit⟩
+                                    fun n n_ih =>
+                                    ⟨(fun x f x_5 =>
+                                          (match (motive :=
+                                              Nat → (x : Nat) → Nat.below (motive := fun x => Nat → Nat) x → Nat) x_5,
+                                              x with
+                                            | a, Nat.zero => fun x => a
+                                            | a, b.succ => fun x => (x.1 a).succ)
+                                            f)
+                                        n.succ n_ih,
+                                      n_ih⟩))))))
+                        (L4L.appArgHEq' (fun f => f n)
+                          (HEq.symm
+                            (L4L.appHEqABUV'
+                              (L4L.appArgHEq' (PProd ((fun x => Nat → Nat) 1))
+                                (HEq.trans (nat_iota_succ PUnit (fun n n_ih => (fun x => Nat → Nat) n ×' n_ih) 0)
+                                  (L4L.appArgHEq' (PProd ((fun x => Nat → Nat) 0))
+                                    (HEq.trans (nat_iota_zero PUnit fun n n_ih => (fun x => Nat → Nat) n ×' n_ih)
+                                      (nat_iota_zero PUnit fun n n_ih => (fun x => Nat → Nat) n ×' n_ih)))))
+                              (fun a a_1 a_2 =>
+                                L4L.HEqRefl
+                                  ((fun β a => (fun x => Nat → Nat) 1) (Nat.below (motive := fun x => Nat → Nat) 1) a))
+                              (L4L.appArgHEq' ((fun α β a => a.1) ((fun x => Nat → Nat) 1))
+                                (HEq.trans (nat_iota_succ PUnit (fun n n_ih => (fun x => Nat → Nat) n ×' n_ih) 0)
+                                  (L4L.appArgHEq' (PProd ((fun x => Nat → Nat) 0))
+                                    (HEq.trans (nat_iota_zero PUnit fun n n_ih => (fun x => Nat → Nat) n ×' n_ih)
+                                      (nat_iota_zero PUnit fun n n_ih => (fun x => Nat → Nat) n ×' n_ih)))))
+                              (nat_iota_succ
+                                ⟨(fun x f x_5 =>
+                                      (match (motive :=
+                                          Nat → (x : Nat) → Nat.below (motive := fun x => Nat → Nat) x → Nat) x_5,
+                                          x with
+                                        | a, Nat.zero => fun x => a
+                                        | a, b.succ => fun x => (x.1 a).succ)
+                                        f)
+                                    Nat.zero PUnit.unit,
+                                  PUnit.unit⟩
+                                (fun n n_ih =>
+                                  ⟨(fun x f x_5 =>
+                                        (match (motive :=
+                                            Nat → (x : Nat) → Nat.below (motive := fun x => Nat → Nat) x → Nat) x_5,
+                                            x with
+                                          | a, Nat.zero => fun x => a
+                                          | a, b.succ => fun x => (x.1 a).succ)
+                                          f)
+                                      n.succ n_ih,
+                                    n_ih⟩)
+                                0))))))
+                    h))))
+        f)
+    x_1 x_2
+-/
+#guard_msgs in
+#patch_const Nat.eq_or_lt_of_le (iotaReduction := iotaReduction) -kLikeReduction -proofIrrelevance
